theories/AlgorithmicTypingProperties.v
@@ -10,7 +10,7 @@ Proof.
   etransitivity ; tea.
   symmetry.
   eapply RedConvTyC, subject_reduction_type ; tea.
-  now eapply validity in Hconv as [].
+  boundary.
 Qed.
 
 Section AlgoConvConv.
@@ -26,8 +26,7 @@ Section AlgoConvConv.
   1: eexists ; split.
   - now econstructor.
   - cbn.
-    eapply typing_shift ; tea.
-    all: eapply validity in H3 as []; gen_typing.
+    eapply typing_shift ; boundary.
   - destruct d as [? d].
     edestruct IHHin as [[? d'] []].
     1: eassumption.
@@ -35,8 +34,7 @@ Section AlgoConvConv.
     econstructor ; split.
     1: now econstructor.
     cbn.
-    eapply typing_shift ; tea.
-    all: now eapply validity in H3 as [] ; gen_typing.
+    eapply typing_shift ; boundary.
   Qed.
 
   Lemma in_ctx_conv_l Γ' Γ n decl' :
@@ -78,7 +76,7 @@ Section AlgoConvConv.
       eexists ; split.
       1: now econstructor.
       eassumption.
-    - intros * ? IHm Ht [IHt []%validity] **.
+    - intros * ? IHm Ht [IHt []%boundary] **.
       edestruct IHm as [[? [? (?&?&?&[HconvP HconvA])%red_ty_compl_prod_r]] ?] ; tea.
       eapply redty_red, red_whnf in HconvP as ->.
       2: gen_typing.
@@ -116,13 +114,13 @@ Section AlgoConvConv.
       2: gen_typing.
       econstructor ; refold.
       + eapply IHA ; tea.
-        do 2 econstructor.
-        now eapply wf_conv_ctx.
+        do 2 econstructor ; refold.
+        boundary.
       + assert [Γ' |-[de] A].
         {
           eapply stability ; tea.
-          econstructor.
-          now eapply validity in HconvA as [].
+          econstructor ; refold.
+          now boundary.
         }
         eapply IHB ; tea.
         all: econstructor ; tea.
@@ -177,10 +175,10 @@ Section AlgoConvConv.
     unshelve (repeat (split ; [destruct Hind as [Hind _] ; shelve | destruct Hind as [_ Hind]])).
     1-2: now constructor.
     all: intros * Hconv ; intros ; eapply Hind ; tea.
-    all: match goal with H : ConvCtx _ _ |- _ => symmetry in H ; apply wf_conv_ctx in H end.
+    all: match goal with H : ConvCtx _ _ |- _ => symmetry in H ; apply boundary_ctx_conv_l in H end.
     all: split ; tea.
     all: try solve [now apply algo_conv_wh in Hconv as []].
-    all: now eapply validity in H2.
+    all: now boundary.
   Qed.
 
 End AlgoConvConv.
@@ -277,10 +275,10 @@ Section Symmetry.
         * now symmetry.
         * eapply stability.
           2: now symmetry.
-          now eapply validity in Hwft as [].
+          boundary.
         * eapply stability.
           2: now symmetry.
-          now eapply validity in Hwft as [].
+          boundary.
       + eapply typing_subst1 ; tea.
         econstructor ; refold.
         2: now symmetry.
@@ -295,7 +293,7 @@ Section Symmetry.
         eapply RedConvTyC, subject_reduction_type ; tea.
         eapply stability.
         2: now symmetry.
-        now eapply validity in Hwf as [].
+        boundary.
       }
       pose proof Hconv' as [? []]%red_ty_complete; tea.
       eexists ; split.
@@ -317,7 +315,7 @@ Section Symmetry.
       1-2: assumption.
       eapply IH.
       econstructor ; tea.
-      eapply validity, prod_ty_inv in Hf as [].
+      eapply boundary, prod_ty_inv in Hf as [].
       now econstructor.
     - intros * ? IH  **.
       edestruct IH as [[? []] []] ; tea.
@@ -414,7 +412,7 @@ Section Transitivity.
       1: now econstructor.
       etransitivity ; [|etransitivity].
       1: symmetry.
-      1,3: eapply RedConvTyC, subject_reduction_type ; tea ; now eapply validity in HconvA.
+      1,3: eapply RedConvTyC, subject_reduction_type ; tea ; boundary.
       eassumption.
     - intros * ? ? Hu Ht' IHt ? ? ? * ? HconvA Hconv.
       inversion Hconv ; subst ; clear Hconv ; refold.
@@ -425,7 +423,7 @@ Section Transitivity.
       eapply IHt ; tea.
       etransitivity ; [|etransitivity].
       1: symmetry.
-      1,3: eapply RedConvTyC, subject_reduction_type ; tea ; now eapply validity in HconvA.
+      1,3: eapply RedConvTyC, subject_reduction_type ; tea ; boundary.
       eassumption.
     - intros * ? [IHA HpostA] ? IHB ? ? ? * HΓ ? Hconv.
       inversion Hconv ; subst ; clear Hconv ; refold.
@@ -437,9 +435,9 @@ Section Transitivity.
       3: eassumption.
       + econstructor ; tea. now econstructor.
       + do 3 econstructor ; refold.
-        * now symmetry in HΓ ; eapply wf_conv_ctx in HΓ.
+        * now symmetry in HΓ ; boundary.
         * econstructor ; refold.
-          now eapply validity in HpostA as [].
+          boundary.
     - intros * ? ? ? IH ? ? ? * ? ? Hconv.
       inversion Hconv ; subst ; clear Hconv ; refold.
       1,3: now unshelve eapply ty_conv_inj in H6 ; [econstructor | econstructor | cbn in *].
@@ -514,8 +512,8 @@ Module AlgorithmicTypingProperties.
       econstructor ; refold ; tea.
       eapply algo_conv_trans.
       + split ; tea.
-        now eapply typing_sound, validity in Ht.
-      + now eapply ctx_conv_refl.
+        now eapply typing_sound, boundary in Ht.
+      + now eapply ctx_refl.
       + eapply HA.
   Qed.
 
@@ -528,12 +526,12 @@ Module AlgorithmicTypingProperties.
     - red ; intros_bn.
       eapply algo_conv_sym.
       + now econstructor.
-      + now eapply ctx_conv_refl. 
+      + now eapply ctx_refl. 
     - red ; intros * Hconv [? ? ? Hconv'].
       econstructor ; tea.
       1: now apply Hconv.
       eapply algo_conv_trans ; tea.
-      now eapply ctx_conv_refl.
+      now eapply ctx_refl.
     - intros_bn.
       1-2: now apply typing_wk.
       now apply algo_conv_wk.
@@ -550,7 +548,7 @@ Module AlgorithmicTypingProperties.
       + econstructor ; tea ; refold.
         eapply stability ; tea.
         econstructor.
-        * now eapply ctx_conv_refl.
+        * now eapply ctx_refl.
         * symmetry.
           now eapply conv_sound in bun_conv_ty0.
       + now do 2 econstructor.
@@ -562,18 +560,18 @@ Module AlgorithmicTypingProperties.
     - red ; intros_bn.
       eapply algo_conv_sym.
       + now econstructor.
-      + now eapply ctx_conv_refl. 
+      + now eapply ctx_refl. 
     - red. intros * Hconv [? ? ? Hconv'].
       split ; tea.
       1: apply Hconv.
       eapply algo_conv_trans ; tea.
-      + now apply ctx_conv_refl.
+      + now apply ctx_refl.
       + now constructor.
     - intros_bn.
       all: eapply conv_sound in bun_conv_ty ; tea.
       1-2: now econstructor.
       eapply algo_conv_conv ; tea.
-      now apply ctx_conv_refl.
+      now apply ctx_refl.
     - intros_bn.
       1-3: now apply typing_wk.
       now apply algo_conv_wk.
@@ -589,25 +587,24 @@ Module AlgorithmicTypingProperties.
         1-3: now etransitivity.
         eassumption.
     - intros Γ n n' A [? ? ? ? ? A' Hconvn HconvA].
-      assert [Γ |-[de] A]
-        by now eapply validity in HconvA as [].
+      assert [Γ |-[de] A] by boundary.
       assert [Γ |-[de] n : A'] by
-        (eapply conv_sound in Hconvn as [[]%validity] ; tea ; now gen_typing).
+        (eapply conv_sound in Hconvn as [[]%boundary] ; tea ; now gen_typing).
       assert [Γ |-[de] n' : A'] by
-        (eapply conv_sound in Hconvn as [[]%validity] ; tea ; now gen_typing).
+        (eapply conv_sound in Hconvn as [[]%boundary] ; tea ; now gen_typing).
       split ; tea.
       1-2: now gen_typing.
       eapply algo_conv_conv ; tea.
-      2: now eapply ctx_conv_refl.
+      2: now eapply ctx_refl.
       apply ne_conv_conv.
       2: eassumption.
-      now eapply validity in HconvA as [].
+      boundary.
     - intros_bn.
       + now constructor.
       + constructor ; tea.
         eapply stability ; tea.
         econstructor.
-        1: now apply ctx_conv_refl.
+        1: now apply ctx_refl.
         eapply conv_sound in bun_conv_tm0 ; tea.
         symmetry.
         now constructor.
@@ -629,14 +626,14 @@ Module AlgorithmicTypingProperties.
         now econstructor.
       }
       eapply algo_conv_sym in Hconv as [? []].
-      2: now eapply ctx_conv_refl.
+      2: now eapply ctx_refl.
       econstructor ; tea.
       etransitivity ; tea.
       now symmetry.
     - red. intros_bn.
       + eapply algo_conv_trans ; tea.
         * now constructor.
-        * now apply ctx_conv_refl.
+        * now apply ctx_refl.
       + eassumption.
     - intros_bn.
       1: eassumption.
@@ -664,22 +661,21 @@ Module AlgorithmicTypingProperties.
       + gen_typing.
       + now econstructor ; refold.
       + eapply conv_sound in H0 ; tea.
-        enough [Γ |-[de] tRel n : decl_type decl] as Hty by
-          now apply validity in Hty.
+        enough [Γ |-[de] tRel n : decl_type decl] by boundary.
         now econstructor.
   - intros *
     [? ? ? ? ? ? Hf (?&?&?&[])%red_ty_compl_prod_r]
     [? ? ? ? Ht].
     econstructor ; tea.
     + eapply conv_sound in Hf as [Hf] ; tea.
-      eapply validity in Hf as [_ Hf _].
+      eapply boundary in Hf as [_ Hf _].
       eexists ; econstructor ; refold.
       * econstructor ; tea.
         now eapply RedConvTyC.
       * now econstructor.
     + gen_typing.
     + eapply conv_sound in Hf as [Hg] ; tea.
-      eapply validity in Hg as [_ _ Hg].
+      eapply boundary in Hg as [_ _ Hg].
       eexists ; econstructor ; refold.
       * econstructor ; tea.
         now eapply RedConvTyC.
@@ -690,10 +686,10 @@ Module AlgorithmicTypingProperties.
         2: econstructor.
         now eapply redty_red.
       * eapply algo_conv_conv ; tea.
-        now eapply ctx_conv_refl.
+        now eapply ctx_refl.
     + eapply typing_subst1 ; tea.
       econstructor.
-      eapply conv_sound, validity in Ht as [] ; tea.
+      eassumption.
   Qed.
 
   #[export, refine] Instance RedTermAlgProperties :
